Update wrt. iris trunk.

lang.v
@@ -42,79 +42,71 @@ Proof.
   induction mxl as [|?? IH]; set_solver.
 Qed.
 
-(** A typeclass for whether a variable is bound in a given
-   context. Making this a typeclass means we can use typeclass search
-   to program solving these constraints, so this becomes extensible.
-   Also, since typeclass search runs *after* unification, Coq has already
-   inferred the X for us; if we were to go for embedded proof terms ot
-   tactics, Coq would do things in the wrong order. *)
-Class VarBound (x : string) (X : list string) :=
-  var_bound : bool_decide (x ∈ X).
-(* There is no need to restrict this hint to terms without evars, [vm_compute]
-will fail in case evars are arround. *)
-Hint Extern 0 (VarBound _ _) => vm_compute; exact I : typeclass_instances.
-
-Instance var_bound_proof_irrel x X : ProofIrrel (VarBound x X).
-Proof. rewrite /VarBound. apply _. Qed.
-Instance set_unfold_var_bound x X P :
-  SetUnfold (x ∈ X) P → SetUnfold (VarBound x X) P.
-Proof.
-  constructor. by rewrite /VarBound bool_decide_spec (set_unfold (x ∈ X) P).
-Qed.
-
-Inductive expr (X : list string) :=
-(* Var is the only place where the terms contain a proof. The fact that they
-   contain a proof at all is suboptimal, since this means two seeminlgy
-   convertible terms could differ in their proofs. However, this also has
-   some advantages:
-   * We can make the [X] an index, so we can do non-dependent match.
-   * In expr_weaken, we can push the proof all the way into Var, making
-     sure that proofs never block computation. *)
-| Var (x : string) `{VarBound x X}
+Inductive expr :=
+| Var (x : string)
 | Lit (l : base_lit)
-| Rec (f : binder) (xl : list binder) (e : expr (xl +b+ f :b: X))
-| BinOp (op : bin_op) (e1 e2 : expr X)
-| App (e : expr X) (el : list (expr X))
-| Read (o : order) (e : expr X)
-| Write (o : order) (e1 e2: expr X)
-| CAS (e0 e1 e2 : expr X)
-| Alloc (e : expr X)
-| Free (e1 e2 : expr X)
-| Case (e : expr X) (el : list (expr X))
-| Fork (e : expr X).
+| Rec (f : binder) (xl : list binder) (e : expr)
+| BinOp (op : bin_op) (e1 e2 : expr)
+| App (e : expr) (el : list expr)
+| Read (o : order) (e : expr)
+| Write (o : order) (e1 e2: expr)
+| CAS (e0 e1 e2 : expr)
+| Alloc (e : expr)
+| Free (e1 e2 : expr)
+| Case (e : expr) (el : list expr)
+| Fork (e : expr).
 
 Bind Scope lrust_expr_scope with expr.
 Bind Scope lrust_expr_scope with list expr.
 Delimit Scope lrust_expr_scope with RustE.
-Arguments Var {_} _ {_}.
-Arguments Lit {_} _.
-Arguments Rec {_} _ _ _%RustE.
-Arguments BinOp {_} _ _%RustE _%RustE.
-Arguments App {_} _%RustE _%RustE.
-Arguments Read {_} _ _%RustE.
-Arguments Write {_} _ _%RustE _%RustE.
-Arguments CAS {_} _%RustE _%RustE _%RustE.
-Arguments Alloc {_} _%RustE.
-Arguments Free {_} _%RustE _%RustE.
-Arguments Case {_} _%RustE _%RustE.
-Arguments Fork {_} _%RustE.
+Arguments Var _.
+Arguments Lit _.
+Arguments Rec _ _ _%RustE.
+Arguments BinOp _ _%RustE _%RustE.
+Arguments App _%RustE _%RustE.
+Arguments Read _ _%RustE.
+Arguments Write _ _%RustE _%RustE.
+Arguments CAS _%RustE _%RustE _%RustE.
+Arguments Alloc _%RustE.
+Arguments Free _%RustE _%RustE.
+Arguments Case _%RustE _%RustE.
+Arguments Fork _%RustE.
+
+Fixpoint is_closed (X : list string) (e : expr) : bool :=
+  match e with
+  | Var x => bool_decide (x ∈ X)
+  | Lit _ => true
+  | Rec f xl e => is_closed (f :b: xl +b+ X) e
+  | BinOp _ e1 e2 | Write _ e1 e2 | Free e1 e2 =>
+    is_closed X e1 && is_closed X e2
+  | App e el | Case e el => is_closed X e && forallb (is_closed X) el
+  | Read _ e | Alloc e | Fork e => is_closed X e
+  | CAS e0 e1 e2 => is_closed X e0 && is_closed X e1 && is_closed X e2
+  end.
+
+Class Closed (X : list string) (e : expr) := closed : is_closed X e.
+Instance closed_proof_irrel env e : ProofIrrel (Closed env e).
+Proof. rewrite /Closed. apply _. Qed.
+Instance closed_decision env e : Decision (Closed env e).
+Proof. rewrite /Closed. apply _. Qed.
 
 Inductive val :=
 | LitV (l : base_lit)
-| RecV (f : binder) (xl : list binder) (e : expr (xl +b+ f :b: [])).
+| RecV (f : binder) (xl : list binder) (e : expr) `{Closed (f :b: xl +b+ []) e}.
 
 Bind Scope lrust_val_scope with val.
 Delimit Scope lrust_val_scope with RustV.
 
-Definition of_val (v : val) : expr [] :=
+Definition of_val (v : val) : expr :=
   match v with
-  | RecV f x e => Rec f x e
+  | RecV f x e _ => Rec f x e
   | LitV l => Lit l
   end.
 
-Definition to_val (e : expr []) : option val :=
+Definition to_val (e : expr) : option val :=
   match e with
-  | Rec f x e => Some (RecV f x e)
+  | Rec f xl e =>
+    if decide (Closed (f :b: xl +b+ []) e) then Some (RecV f xl e) else None
   | Lit l => Some (LitV l)
   | _ => None
   end.
@@ -126,22 +118,22 @@ Definition state := gmap loc (lock_state * val).
 
 (** Evaluation contexts *)
 Inductive ectx_item :=
-| BinOpLCtx (op : bin_op) (e2 : expr [])
+| BinOpLCtx (op : bin_op) (e2 : expr)
 | BinOpRCtx (op : bin_op) (v1 : val)
-| AppLCtx (e2 : list (expr []))
-| AppRCtx (v : val) (vl : list val) (el : list (expr []))
+| AppLCtx (e2 : list expr)
+| AppRCtx (v : val) (vl : list val) (el : list expr)
 | ReadCtx (o : order)
-| WriteLCtx (o : order) (e2 : expr [])
+| WriteLCtx (o : order) (e2 : expr)
 | WriteRCtx (o : order) (v1 : val)
-| CasLCtx (e1 e2: expr [])
-| CasMCtx (v0 : val) (e2 : expr [])
+| CasLCtx (e1 e2: expr)
+| CasMCtx (v0 : val) (e2 : expr)
 | CasRCtx (v0 : val) (v1 : val)
 | AllocCtx
-| FreeLCtx (e2 : expr [])
+| FreeLCtx (e2 : expr)
 | FreeRCtx (v1 : val)
-| CaseCtx (el : list (expr [])).
+| CaseCtx (el : list expr).
 
-Definition fill_item (Ki : ectx_item) (e : expr []) : expr [] :=
+Definition fill_item (Ki : ectx_item) (e : expr) : expr :=
   match Ki with
   | BinOpLCtx op e2 => BinOp op e e2
   | BinOpRCtx op v1 => BinOp op (of_val v1) e
@@ -160,65 +152,26 @@ Definition fill_item (Ki : ectx_item) (e : expr []) : expr [] :=
   end.
 
 (** Substitution *)
-Program Fixpoint wexpr {X Y} (H : X `included` Y) (e : expr X) : expr Y :=
-  match e return expr Y with
-  | Var x _ => @Var _ x _
-  | Lit l => Lit l
-  | Rec f xl e => Rec f xl (wexpr _ e)
-  | BinOp op e1 e2 => BinOp op (wexpr H e1) (wexpr H e2)
-  | App e el => App (wexpr H e) (map (wexpr H) el)
-  | Read o e => Read o (wexpr H e)
-  | Write o e1 e2 => Write o (wexpr H e1) (wexpr H e2)
-  | CAS e0 e1 e2 => CAS (wexpr H e0) (wexpr H e1) (wexpr H e2)
-  | Alloc e => Alloc (wexpr H e)
-  | Free e1 e2 => Free (wexpr H e1) (wexpr H e2)
-  | Case e el => Case (wexpr H e) (map (wexpr H) el)
-  | Fork e => Fork (wexpr H e)
-  end.
-Solve Obligations with set_solver.
-
-Definition wexpr' {X} (e : expr []) : expr X := wexpr (included_nil _) e.
-
-Definition of_val' {X} (v : val) : expr X := wexpr (included_nil _) (of_val v).
-
-Lemma wsubst_rec_true_prf {X Y x} (H : X `included` x :: Y)
-      {f} {xl : list binder} (Hfxl : BNamed x ≠ f ∧ BNamed x ∉ xl) :
-  xl +b+ f :b: X `included` x :: xl +b+ f :b: Y.
-Proof. set_solver. Qed.
-
-Lemma wsubst_rec_false_prf {X Y x} (H : X `included` x :: Y)
-      {f} {xl : list binder} (Hfxl : ¬ (BNamed x ≠ f ∧ BNamed x ∉ xl)) :
-  xl +b+ f :b: X `included` xl +b+ f :b: Y.
-Proof. move: Hfxl=>/not_and_l [/dec_stable|/dec_stable]; set_solver. Qed.
-
-Program Fixpoint wsubst {X Y} (x : string) (es : expr [])
-    (H : X `included` x :: Y) (e : expr X)  : expr Y :=
-  match e return expr Y with
-  | Var y _ => if decide (x = y) then wexpr' es else @Var _ y _
+Fixpoint subst (x : string) (es : expr) (e : expr)  : expr :=
+  match e with
+  | Var y => if bool_decide (y = x) then es else Var y
   | Lit l => Lit l
   | Rec f xl e =>
-     Rec f xl $ match decide (BNamed x ≠ f ∧ BNamed x ∉ xl) return _ with
-                | left Hfy => wsubst x es (wsubst_rec_true_prf H Hfy) e
-                | right Hfy => wexpr (wsubst_rec_false_prf H Hfy) e
-                end
-  | BinOp op e1 e2 => BinOp op (wsubst x es H e1) (wsubst x es H e2)
-  | App e el => App (wsubst x es H e) (map (wsubst x es H) el)
-  | Read o e => Read o (wsubst x es H e)
-  | Write o e1 e2 => Write o (wsubst x es H e1) (wsubst x es H e2)
-  | CAS e0 e1 e2 => CAS (wsubst x es H e0) (wsubst x es H e1) (wsubst x es H e2)
-  | Alloc e => Alloc (wsubst x es H e)
-  | Free e1 e2 => Free (wsubst x es H e1) (wsubst x es H e2)
-  | Case e el => Case (wsubst x es H e) (map (wsubst x es H) el)
-  | Fork e => Fork (wsubst x es H e)
+    Rec f xl $ if bool_decide (BNamed x ≠ f ∧ BNamed x ∉ xl) then subst x es e else e
+  | BinOp op e1 e2 => BinOp op (subst x es e1) (subst x es e2)
+  | App e el => App (subst x es e) (map (subst x es) el)
+  | Read o e => Read o (subst x es e)
+  | Write o e1 e2 => Write o (subst x es e1) (subst x es e2)
+  | CAS e0 e1 e2 => CAS (subst x es e0) (subst x es e1) (subst x es e2)
+  | Alloc e => Alloc (subst x es e)
+  | Free e1 e2 => Free (subst x es e1) (subst x es e2)
+  | Case e el => Case (subst x es e) (map (subst x es) el)
+  | Fork e => Fork (subst x es e)
   end.
-Solve Obligations with set_solver.
 
-Definition subst {X} (x : string) (es : expr []) (e : expr (x :: X)) : expr X :=
-  wsubst x es (λ z, id) e.
-Definition subst' {X} (mx : binder) (es : expr []) : expr (mx :b: X) → expr X :=
+Definition subst' (mx : binder) (es : expr) : expr → expr :=
   match mx with BNamed x => subst x es | BAnon => id end.
-Fixpoint subst_l {X} (xl : list binder) (esl : list (expr [])) :
-                     expr (xl +b+ X) → option (expr X) :=
+Fixpoint subst_l (xl : list binder) (esl : list expr) : expr → option expr :=
   match xl, esl with
   | [], [] => λ e, Some e
   | x::xl, es::esl => λ e, subst_l xl esl (subst' x es e)
@@ -266,23 +219,24 @@ Definition value_eq (σ : state) (v1 v2 : val) : option bool :=
   | _, _ => None
   end.
 
-Inductive head_step : expr [] → state → expr [] → state → option (expr []) → Prop :=
+Inductive head_step : expr → state → expr → state → option expr → Prop :=
 | BinOpS op l1 l2 l' σ :
     bin_op_eval op l1 l2 = Some l' →
     head_step (BinOp op (Lit l1) (Lit l2)) σ (Lit l') σ None
 | BetaS f xl e e' el σ:
     Forall (λ ei, is_Some (to_val ei)) el →
+    Closed (f :b: xl +b+ []) e →
     subst_l xl el e = Some e' →
     head_step (App (Rec f xl e) el) σ (subst' f (Rec f xl e) e') σ None
 | ReadScS l n v σ:
     σ !! l = Some (RSt n, v) →
     head_step (Read ScOrd (Lit $ LitLoc l)) σ (of_val v) σ None
-| ReadNaS l n v σ:
+| ReadNa1S l n v σ:
     σ !! l = Some (RSt n, v) →
     head_step (Read Na1Ord (Lit $ LitLoc l)) σ
               (Read Na2Ord (Lit $ LitLoc l)) (<[l:=(RSt $ S n, v)]>σ)
               None
-| ReadInS l n v σ:
+| ReadNa2S l n v σ:
     σ !! l = Some (RSt $ S n, v) →
     head_step (Read Na2Ord (Lit $ LitLoc l)) σ
               (of_val v) (<[l:=(RSt n, v)]>σ)
@@ -293,20 +247,20 @@ Inductive head_step : expr [] → state → expr [] → state → option (expr [
     head_step (Write ScOrd (Lit $ LitLoc l) e) σ
               (Lit LitUnit) (<[l:=(RSt 0, v)]>σ)
               None
-| WriteNaS l e v' σ:
-    is_Some (to_val e) →
+| WriteNa1S l e v v' σ:
+    to_val e = Some v →
     σ !! l = Some (RSt 0, v') →
     head_step (Write Na1Ord (Lit $ LitLoc l) e) σ
               (Write Na2Ord (Lit $ LitLoc l) e) (<[l:=(WSt, v')]>σ)
               None
-| WriteInS l e v v' σ:
+| WriteNa2S l e v v' σ:
     to_val e = Some v →
     σ !! l = Some (WSt, v') →
     head_step (Write Na2Ord (Lit $ LitLoc l) e) σ
               (Lit LitUnit) (<[l:=(RSt 0, v)]>σ)
               None
-| CasFailS l n e1 v1 e2 vl σ :
-    to_val e1 = Some v1 → is_Some (to_val e2) →
+| CasFailS l n e1 v1 e2 v2 vl σ :
+    to_val e1 = Some v1 → to_val e2 = Some v2 →
     σ !! l = Some (RSt n, vl) →
     value_eq σ v1 vl = Some false →
     head_step (CAS (Lit $ LitLoc l) e1 e2) σ (Lit $ lit_of_bool false) σ  None
@@ -336,106 +290,15 @@ Inductive head_step : expr [] → state → expr [] → state → option (expr [
 | ForkS e σ:
     head_step (Fork e) σ (Lit LitUnit) σ (Some e).
 
-(** Atomic expressions *)
-Definition atomic (e: expr []) : bool :=
-  match e with
-  | Read (ScOrd | Na2Ord) e | Alloc e => bool_decide (is_Some (to_val e))
-  | Write (ScOrd | Na2Ord) e1 e2 | Free e1 e2 =>
-    bool_decide (is_Some (to_val e1) ∧ is_Some (to_val e2))
-  | CAS e0 e1 e2 =>
-    bool_decide (is_Some (to_val e0) ∧ is_Some (to_val e1) ∧ is_Some (to_val e2))
-  | _ => false
-  end.
-
-(** Substitution *)
-Lemma var_proof_irrel X x H1 H2 : @Var X x H1 = @Var X x H2.
-Proof. f_equal. by apply (proof_irrel _). Qed.
-
-Lemma wexpr_id X (H : X `included` X) e : wexpr H e = e.
-Proof.
-  revert X H e; fix 3.
-  destruct e as [| | | |? el| | | | | |? el|]; f_equal/=;
-    auto using proof_irrel;
-  induction el; f_equal/=; auto.
-Qed.
-Lemma wexpr_proof_irrel X Y (H1 H2 : X `included` Y) e : wexpr H1 e = wexpr H2 e.
-Proof.
-  revert X Y H1 H2 e; fix 5.
-  destruct e as [| | | |? el| | | | | |? el|]; f_equal/=;
-    auto using proof_irrel;
-  induction el; f_equal/=; auto.
-Qed.
-Lemma wexpr_wexpr X Y Z (H1 : X `included` Y) (H2 : Y `included` Z) H3 e :
-  wexpr H2 (wexpr H1 e) = wexpr H3 e.
-Proof.
-  revert X Y Z H1 H2 H3 e; fix 7.
-  destruct e as [| | | |? el| | | | | |? el|]; f_equal/=;
-    auto using proof_irrel;
-  induction el; f_equal/=; auto.
-Qed.
-Lemma wexpr_wexpr' X Y Z (H1 : X `included` Y) (H2 : Y `included` Z) e :
-  wexpr H2 (wexpr H1 e) = wexpr (transitivity H1 H2) e.
-Proof. apply wexpr_wexpr. Qed.
-
-Lemma wsubst_proof_irrel X Y x es (H1 H2 : X `included` x :: Y) e :
-  wsubst x es H1 e = wsubst x es H2 e.
-Proof.
-  revert X Y H1 H2 e; fix 5.
-  destruct e as [| | | |? el| | | | | |? el|];
-    simpl; intros; try case_decide; f_equal;
-    auto using proof_irrel, wexpr_proof_irrel;
-  induction el; f_equal/=; auto.
-Qed.
-Lemma wexpr_wsubst X Y Z x es (H1: X `included` x::Y) (H2: Y `included` Z) H3 e:
-  wexpr H2 (wsubst x es H1 e) = wsubst x es H3 e.
-Proof.
-  revert X Y Z H1 H2 H3 e; fix 7.
-  destruct e; intros; rewrite /=/wexpr'/=; try case_decide; f_equal; simpl;
-    auto using var_proof_irrel, wexpr_wexpr;
-  induction el; f_equal/=; auto.
-Qed.
-Lemma wsubst_wexpr X Y Z x es (H1: X `included` Y) (H2: Y `included` x::Z) H3 e:
-  wsubst x es H2 (wexpr H1 e) = wsubst x es H3 e.
-Proof.
-  revert X Y Z H1 H2 H3 e; fix 7.
-  destruct e as [| | | |? el| | | | | |? el|];
-    intros; simpl; try case_decide; f_equal;
-    auto using proof_irrel, wexpr_wexpr;
-  induction el; f_equal/=; auto.
-Qed.
-Lemma wsubst_wexpr' X Y Z x es (H1: X `included` Y) (H2: Y `included` x::Z) e:
-  wsubst x es H2 (wexpr H1 e) = wsubst x es (transitivity H1 H2) e.
-Proof. apply wsubst_wexpr. Qed.
-
-Lemma wsubst_closed X Y x es (H1 : X `included` x :: Y) H2 (e : expr X) :
-  x ∉ X → wsubst x es H1 e = wexpr H2 e.
-Proof.
-  revert X Y H1 H2 e; fix 5.
-  destruct e as [| | | |? el| | | | | |? el|];
-    intros; rewrite /=/wexpr'/=; try case_decide; f_equal;
-    auto using proof_irrel, wexpr_proof_irrel with set_solver;
-    try (induction el; f_equal/=; auto).
-  clear wsubst_closed. exfalso; set_solver.
-Qed.
-Lemma wsubst_closed_nil x es H (e : expr []) : wsubst x es H e = e.
-Proof.
-  rewrite -{2}(wexpr_id _ (reflexivity []) e).
-  apply wsubst_closed, not_elem_of_nil.
-Qed.
-
 (** Basic properties about the language *)
 Lemma to_of_val v : to_val (of_val v) = Some v.
-Proof. by induction v; simplify_option_eq. Qed.
+Proof.
+  by induction v; simplify_option_eq; repeat f_equal; try apply (proof_irrel _).
+Qed.
 
 Lemma of_to_val e v : to_val e = Some v → of_val v = e.
 Proof.
-  revert e v. cut (∀ X (e : expr X) (H : X = ∅) v,
-    to_val (eq_rect _ expr e _ H) = Some v → of_val v = eq_rect _ expr e _ H).
-  { intros help e v. apply (help ∅ e eq_refl). }
-  intros X e; induction e; intros HX ??; simplify_option_eq;
-    repeat match goal with
-    | IH : ∀ _ : ∅ = ∅, _ |- _ => specialize (IH eq_refl); simpl in IH
-    end; auto with f_equal.
+  revert v; induction e; intros v ?; simplify_option_eq; auto with f_equal.
 Qed.
 
 Instance of_val_inj : Inj (=) (=) of_val.
@@ -452,23 +315,12 @@ Lemma val_stuck e1 σ1 e2 σ2 ef :
   head_step e1 σ1 e2 σ2 ef → to_val e1 = None.
 Proof. destruct 1; naive_solver. Qed.
 
-Lemma atomic_not_val e : atomic e → to_val e = None.
-Proof. by destruct e. Qed.
-
-Lemma atomic_fill_item Ki e : atomic (fill_item Ki e) → is_Some (to_val e).
-Proof.
-  by intros; destruct Ki; repeat (case_match || simplify_eq/= || destruct_and?).
-Qed.
-
-Lemma atomic_step e1 σ1 e2 σ2 ef :
-  atomic e1 → head_step e1 σ1 e2 σ2 ef → is_Some (to_val e2).
-Proof.
-  by destruct 2; simpl; rewrite ?to_of_val; eauto.
-Qed.
-
 Lemma head_ctx_step_val Ki e σ1 e2 σ2 ef :
   head_step (fill_item Ki e) σ1 e2 σ2 ef → is_Some (to_val e).
-Proof. destruct Ki; inversion_clear 1; eauto. by decompose_Forall_hyps. Qed.
+Proof.
+  destruct Ki; inversion_clear 1; decompose_Forall_hyps;
+    simplify_option_eq; by eauto.
+Qed.
 
 Lemma list_expr_val_eq_inv vl1 vl2 e1 e2 el1 el2 :
   to_val e1 = None → to_val e2 = None →
@@ -524,6 +376,37 @@ Proof.
   - rewrite repeat_length. apply Z2Nat.id. lia.
 Qed.
 
+(** Closed expressions *)
+Lemma is_closed_weaken X Y e : is_closed X e → X `included` Y → is_closed Y e.
+Proof.
+  revert e X Y. fix 1; destruct e=>X Y/=; try naive_solver.
+  - naive_solver set_solver.
+  - rewrite !andb_True. intros [He Hel] HXY. split. by eauto.
+    induction el=>/=; naive_solver.
+  - rewrite !andb_True. intros [He Hel] HXY. split. by eauto.
+    induction el=>/=; naive_solver.
+Qed.
+
+Lemma is_closed_weaken_nil X e : is_closed [] e → is_closed X e.
+Proof. intros. by apply is_closed_weaken with [], included_nil. Qed.
+
+Lemma is_closed_subst X e x es : is_closed X e → x ∉ X → subst x es e = e.
+Proof.
+  revert e X. fix 1; destruct e=> X /=; rewrite ?bool_decide_spec ?andb_True=> He ?;
+    repeat case_bool_decide; simplify_eq/=; f_equal;
+    try by intuition eauto with set_solver.
+  - case He=> _. clear He. induction el=>//=. rewrite andb_True=>?.
+    f_equal; intuition eauto with set_solver.
+  - case He=> _. clear He. induction el=>//=. rewrite andb_True=>?.
+    f_equal; intuition eauto with set_solver.
+Qed.
+
+Lemma is_closed_nil_subst e x es : is_closed [] e → subst x es e = e.
+Proof. intros. apply is_closed_subst with []; set_solver. Qed.
+
+Lemma is_closed_of_val X v : is_closed X (of_val v).
+Proof. apply is_closed_weaken_nil. induction v; simpl; auto. Qed.
+
 (** Equality and other typeclass stuff *)
 Instance base_lit_dec_eq (l1 l2 : base_lit) : Decision (l1 = l2).
 Proof. solve_decision. Defined.
@@ -532,7 +415,7 @@ Proof. solve_decision. Defined.
 Instance un_op_dec_eq (ord1 ord2 : order) : Decision (ord1 = ord2).
 Proof. solve_decision. Defined.
 
-Fixpoint expr_beq {X Y} (e : expr X) (e' : expr Y) : bool :=
+Fixpoint expr_beq (e : expr) (e' : expr) : bool :=
   let fix expr_list_beq el el' :=
     match el, el' with
     | [], [] => true
@@ -541,7 +424,7 @@ Fixpoint expr_beq {X Y} (e : expr X) (e' : expr Y) : bool :=
     end
   in
   match e, e' with
-  | Var x _, Var x' _ => bool_decide (x = x')
+  | Var x, Var x' => bool_decide (x = x')
   | Lit l, Lit l' => bool_decide (l = l')
   | Rec f xl e, Rec f' xl' e' =>
     bool_decide (f = f') && bool_decide (xl = xl') && expr_beq e e'
@@ -558,25 +441,23 @@ Fixpoint expr_beq {X Y} (e : expr X) (e' : expr Y) : bool :=
   | Free e1 e2, Free e1' e2' => expr_beq e1 e1' && expr_beq e2 e2'
   | _, _ => false
   end.
-Lemma expr_beq_correct {X} (e1 e2 : expr X) : expr_beq e1 e2 ↔ e1 = e2.
+Lemma expr_beq_correct (e1 e2 : expr) : expr_beq e1 e2 ↔ e1 = e2.
 Proof.
-  revert X e1 e2; fix 2;
+  revert e1 e2; fix 1;
     destruct e1 as [| | | |? el1| | | | | |? el1|],
              e2 as [| | | |? el2| | | | | |? el2|]; simpl; try done;
   rewrite ?andb_True ?bool_decide_spec ?expr_beq_correct;
   try (split; intro; [destruct_and?|split_and?]; congruence).
-  - split; intro. subst. apply var_proof_irrel. congruence.
-  - specialize (expr_beq_correct _ e1). naive_solver.
   - match goal with |- context [?F el1 el2] => assert (F el1 el2 ↔ el1 = el2) end.
     { revert el2. induction el1 as [|el1h el1q]; destruct el2; try done.
-      specialize (expr_beq_correct _ el1h). naive_solver. }
+      specialize (expr_beq_correct el1h). naive_solver. }
     clear expr_beq_correct. naive_solver.
   - match goal with |- context [?F el1 el2] => assert (F el1 el2 ↔ el1 = el2) end.
     { revert el2. induction el1 as [|el1h el1q]; destruct el2; try done.
-      specialize (expr_beq_correct _ el1h). naive_solver. }
+      specialize (expr_beq_correct el1h). naive_solver. }
     clear expr_beq_correct. naive_solver.
 Qed.
-Instance expr_dec_eq {X} (e1 e2 : expr X) : Decision (e1 = e2).
+Instance expr_dec_eq (e1 e2 : expr) : Decision (e1 = e2).
 Proof.
  refine (cast_if (decide (expr_beq e1 e2))); by rewrite -expr_beq_correct.
 Defined.
@@ -585,23 +466,20 @@ Proof.
  refine (cast_if (decide (of_val v1 = of_val v2))); abstract naive_solver.
 Defined.
 
-Instance expr_inhabited X : Inhabited (expr X) := populate (Lit LitUnit).
+Instance expr_inhabited : Inhabited expr := populate (Lit LitUnit).
 Instance val_inhabited : Inhabited val := populate (LitV LitUnit).
 
 Canonical Structure stateC := leibnizC state.
 Canonical Structure valC := leibnizC val.
-Canonical Structure exprC X := leibnizC (expr X).
+Canonical Structure exprC := leibnizC expr.
 
 (** Language *)
-Program Instance lrust_ectxi_lang: EctxiLanguage (expr []) val ectx_item state :=
+Program Instance lrust_ectxi_lang: EctxiLanguage expr val ectx_item state :=
   {| ectxi_language.of_val := of_val;
      ectxi_language.to_val := to_val;
      ectxi_language.fill_item := fill_item;
-     ectxi_language.atomic := atomic;
      ectxi_language.head_step := head_step |}.
 Solve Obligations with eauto using to_of_val, of_to_val,
-  val_stuck, atomic_not_val, atomic_step,
-  fill_item_val, atomic_fill_item,
-  fill_item_no_val_inj, head_ctx_step_val.
+  val_stuck, fill_item_val, fill_item_no_val_inj, head_ctx_step_val.
 
-Canonical Structure lrust_lang := ectx_lang (expr []).
+Canonical Structure lrust_lang := ectx_lang expr.
